formal/fstar/ocaml-output/RDF_Indexed.ml
@@ -1,0 +1,69 @@
+open Prims
+type 'a bucket_map = (Prims.string * 'a Prims.list) Prims.list
+let rec bucket_lookup : 'a . 'a bucket_map -> Prims.string -> 'a Prims.list =
+  fun m k ->
+    match m with
+    | [] -> []
+    | (k', v)::rest -> if k = k' then v else bucket_lookup rest k
+let rec bucket_replace_acc :
+  'a .
+    'a bucket_map ->
+      'a bucket_map -> Prims.string -> 'a Prims.list -> 'a bucket_map
+  =
+  fun acc m k v ->
+    match m with
+    | [] -> FStar_List_Tot_Base.rev_acc acc [(k, v)]
+    | (k', v')::rest ->
+        if k = k'
+        then FStar_List_Tot_Base.rev_acc acc ((k, v) :: rest)
+        else bucket_replace_acc ((k', v') :: acc) rest k v
+let bucket_replace (m : 'a bucket_map) (k : Prims.string) (v : 'a Prims.list)
+  : 'a bucket_map= bucket_replace_acc [] m k v
+let bucket_push (m : 'a bucket_map) (k : Prims.string) (t : 'a) :
+  'a bucket_map= bucket_replace m k (t :: (bucket_lookup m k))
+let cmp_by_key (key_of : 'a -> Prims.string FStar_Pervasives_Native.option)
+  (t1 : 'a) (t2 : 'a) : Prims.int=
+  match ((key_of t1), (key_of t2)) with
+  | (FStar_Pervasives_Native.None, FStar_Pervasives_Native.None) ->
+      Prims.int_zero
+  | (FStar_Pervasives_Native.None, FStar_Pervasives_Native.Some uu___) ->
+      (Prims.of_int (-1))
+  | (FStar_Pervasives_Native.Some uu___, FStar_Pervasives_Native.None) ->
+      Prims.int_one
+  | (FStar_Pervasives_Native.Some k1, FStar_Pervasives_Native.Some k2) ->
+      FStar_String.compare k1 k2
+let rec group_sorted_aux :
+  'a .
+    ('a -> Prims.string FStar_Pervasives_Native.option) ->
+      'a Prims.list ->
+        Prims.string FStar_Pervasives_Native.option ->
+          'a Prims.list -> 'a bucket_map -> 'a bucket_map
+  =
+  fun key_of ts cur_key cur_bucket acc ->
+    match ts with
+    | [] ->
+        (match cur_key with
+         | FStar_Pervasives_Native.Some k -> (k, cur_bucket) :: acc
+         | FStar_Pervasives_Native.None -> acc)
+    | t::rest ->
+        (match key_of t with
+         | FStar_Pervasives_Native.None ->
+             group_sorted_aux key_of rest cur_key cur_bucket acc
+         | FStar_Pervasives_Native.Some k ->
+             (match cur_key with
+              | FStar_Pervasives_Native.Some k0 ->
+                  if k = k0
+                  then
+                    group_sorted_aux key_of rest cur_key (t :: cur_bucket)
+                      acc
+                  else
+                    group_sorted_aux key_of rest
+                      (FStar_Pervasives_Native.Some k) [t] ((k0, cur_bucket)
+                      :: acc)
+              | FStar_Pervasives_Native.None ->
+                  group_sorted_aux key_of rest
+                    (FStar_Pervasives_Native.Some k) [t] acc))
+let build_bucket (key_of : 'a -> Prims.string FStar_Pervasives_Native.option)
+  (ts : 'a Prims.list) : 'a bucket_map=
+  let sorted = FStar_List_Tot_Base.sortWith (cmp_by_key key_of) ts in
+  group_sorted_aux key_of sorted FStar_Pervasives_Native.None [] []
