formal/fstar/ocaml-output/RDF_Vocabulary.ml
@@ -1,0 +1,83 @@
+open Prims
+let rdf_type : Prims.string=
+  "http://www.w3.org/1999/02/22-rdf-syntax-ns#type"
+let rdf_Property : Prims.string=
+  "http://www.w3.org/1999/02/22-rdf-syntax-ns#Property"
+let rdf_List : Prims.string=
+  "http://www.w3.org/1999/02/22-rdf-syntax-ns#List"
+let rdf_Statement : Prims.string=
+  "http://www.w3.org/1999/02/22-rdf-syntax-ns#Statement"
+let rdf_first : Prims.string=
+  "http://www.w3.org/1999/02/22-rdf-syntax-ns#first"
+let rdf_rest : Prims.string=
+  "http://www.w3.org/1999/02/22-rdf-syntax-ns#rest"
+let rdf_nil : Prims.string= "http://www.w3.org/1999/02/22-rdf-syntax-ns#nil"
+let rdf_subject : Prims.string=
+  "http://www.w3.org/1999/02/22-rdf-syntax-ns#subject"
+let rdf_predicate : Prims.string=
+  "http://www.w3.org/1999/02/22-rdf-syntax-ns#predicate"
+let rdf_object : Prims.string=
+  "http://www.w3.org/1999/02/22-rdf-syntax-ns#object"
+let rdf_value : Prims.string=
+  "http://www.w3.org/1999/02/22-rdf-syntax-ns#value"
+let rdf_Alt : Prims.string= "http://www.w3.org/1999/02/22-rdf-syntax-ns#Alt"
+let rdf_Bag : Prims.string= "http://www.w3.org/1999/02/22-rdf-syntax-ns#Bag"
+let rdf_Seq : Prims.string= "http://www.w3.org/1999/02/22-rdf-syntax-ns#Seq"
+let rdf_1 : Prims.string= "http://www.w3.org/1999/02/22-rdf-syntax-ns#_1"
+let rdf_2 : Prims.string= "http://www.w3.org/1999/02/22-rdf-syntax-ns#_2"
+let rdf_3 : Prims.string= "http://www.w3.org/1999/02/22-rdf-syntax-ns#_3"
+let rdf_4 : Prims.string= "http://www.w3.org/1999/02/22-rdf-syntax-ns#_4"
+let rdf_5 : Prims.string= "http://www.w3.org/1999/02/22-rdf-syntax-ns#_5"
+let rdfs_subClassOf : Prims.string=
+  "http://www.w3.org/2000/01/rdf-schema#subClassOf"
+let rdfs_subPropertyOf : Prims.string=
+  "http://www.w3.org/2000/01/rdf-schema#subPropertyOf"
+let rdfs_domain : Prims.string= "http://www.w3.org/2000/01/rdf-schema#domain"
+let rdfs_range : Prims.string= "http://www.w3.org/2000/01/rdf-schema#range"
+let rdfs_Class : Prims.string= "http://www.w3.org/2000/01/rdf-schema#Class"
+let rdfs_Resource : Prims.string=
+  "http://www.w3.org/2000/01/rdf-schema#Resource"
+let rdfs_Literal : Prims.string=
+  "http://www.w3.org/2000/01/rdf-schema#Literal"
+let rdfs_Datatype : Prims.string=
+  "http://www.w3.org/2000/01/rdf-schema#Datatype"
+let rdfs_ContainerMembershipProperty : Prims.string=
+  "http://www.w3.org/2000/01/rdf-schema#ContainerMembershipProperty"
+let rdfs_member : Prims.string= "http://www.w3.org/2000/01/rdf-schema#member"
+let rdfs_Container : Prims.string=
+  "http://www.w3.org/2000/01/rdf-schema#Container"
+let rdfs_seeAlso : Prims.string=
+  "http://www.w3.org/2000/01/rdf-schema#seeAlso"
+let rdfs_isDefinedBy : Prims.string=
+  "http://www.w3.org/2000/01/rdf-schema#isDefinedBy"
+let rdfs_comment : Prims.string=
+  "http://www.w3.org/2000/01/rdf-schema#comment"
+let rdfs_label : Prims.string= "http://www.w3.org/2000/01/rdf-schema#label"
+let owl_intersectionOf : Prims.string=
+  "http://www.w3.org/2002/07/owl#intersectionOf"
+let owl_unionOf : Prims.string= "http://www.w3.org/2002/07/owl#unionOf"
+let owl_complementOf : Prims.string=
+  "http://www.w3.org/2002/07/owl#complementOf"
+let owl_disjointWith : Prims.string=
+  "http://www.w3.org/2002/07/owl#disjointWith"
+let owl_Restriction : Prims.string=
+  "http://www.w3.org/2002/07/owl#Restriction"
+let owl_onProperty : Prims.string= "http://www.w3.org/2002/07/owl#onProperty"
+let owl_someValuesFrom : Prims.string=
+  "http://www.w3.org/2002/07/owl#someValuesFrom"
+let owl_allValuesFrom : Prims.string=
+  "http://www.w3.org/2002/07/owl#allValuesFrom"
+let owl_hasValue : Prims.string= "http://www.w3.org/2002/07/owl#hasValue"
+let owl_cardinality : Prims.string=
+  "http://www.w3.org/2002/07/owl#cardinality"
+let owl_minCardinality : Prims.string=
+  "http://www.w3.org/2002/07/owl#minCardinality"
+let owl_maxCardinality : Prims.string=
+  "http://www.w3.org/2002/07/owl#maxCardinality"
+let owl_qualifiedCardinality : Prims.string=
+  "http://www.w3.org/2002/07/owl#qualifiedCardinality"
+let owl_minQualifiedCardinality : Prims.string=
+  "http://www.w3.org/2002/07/owl#minQualifiedCardinality"
+let owl_maxQualifiedCardinality : Prims.string=
+  "http://www.w3.org/2002/07/owl#maxQualifiedCardinality"
+let owl_onClass : Prims.string= "http://www.w3.org/2002/07/owl#onClass"
