formal/fstar/build-ocaml-serializer.sh
@@ -38,8 +38,8 @@ mkdir -p "$BINDIR"
 
 cd "$OUTDIR"
 
-COMMON_MODULES="RDF_Format.ml RDF_Graph_Executable.ml \
-  Parser_FastString.ml Parser_IRI.ml \
+COMMON_MODULES="RDF_Format.ml RDF_Vocabulary.ml RDF_Indexed.ml RDF_Graph_Executable.ml RDF_Vocabulary_Axioms.ml \
+  Parser_FastString.ml RDF_IRI.ml Parser_IRI.ml \
   RDF_NQuads_Serialize.ml \
   Parser_Combinators.ml Parser_TurtleScanner.ml Parser_NTriples.ml Parser_Turtle.ml \
   RDF_Turtle_Serialize.ml \
